experiments/pointless.v
@@ -1,0 +1,344 @@
+From Coq Require Import ssreflect ssrfun ssrbool.
+Require Import stdpp.tactics.
+Require Import stdpp.finite.
+
+Require Import depleted.proset.
+Require Import depleted.bounds.
+Require Import depleted.adjunction.
+Require Import depleted.monoidal.
+Local Open Scope proset_scope.
+Local Open Scope proset_util_scope.
+
+
+Class Frame (X : Type)
+      `{Proset X, !SupLattice X, !MeetSemilattice X, !Exponents X}.
+Hint Mode Frame ! - - - - - : typeclass_instances.
+Instance frame_def `{Proset X, !SupLattice X, !MeetSemilattice X, !Exponents X}
+  : Frame X := {}.
+
+Class FrameMorph `{Proset X, Proset Y} (F : X -> Y)
+      `{!Monotone F, !Cocontinuous F, !Lex F}.
+Hint Mode FrameMorph ! - - ! - - ! - - - : typeclass_instances.
+Instance frame_morph_def `{Proset X, Proset Y} {F : X -> Y}
+         `{!Monotone F, !Cocontinuous F, !Lex F}
+  : FrameMorph F := {}.
+Class FrameMorphPacked `{Proset X, Proset Y} (F : X -> Y) :=
+  {frame_morph_mono :> Monotone F;
+   frame_morph_cocont :> Cocontinuous F;
+   frame_morph_lex :> Lex F}.
+Hint Mode FrameMorphPacked ! - - ! - - ! : typeclass_instances.
+(* This is not an instance in order to avoid loops in resolution. *)
+Definition FMP `{FrameMorph X Y F} : FrameMorphPacked F.
+Proof. constructor; typeclasses eauto. Defined.
+
+(*
+Class HasOpen (X : Type) := Open : Type.
+Arguments Open X {_}.
+Class Locale (X : Type) `{HasOpen X, Frame (Open X)}.
+Hint Mode Locale ! - - - - - - - : typeclass_instances.
+*)
+
+Definition Map (X Y : Type) `{Proset X, Proset Y} : Type :=
+  @sig (Y -> X) FrameMorphPacked.
+Definition preimage (X Y : Type) `{Proset X, Proset Y} : Map X Y -> Y -> X
+  := sval.
+Arguments preimage {_ _ _ _ _ _} !_.
+Instance: Params (@preimage) 6 := {}.
+Notation "f ⁻¹" := (preimage f) (at level 1, format "f ⁻¹").
+Instance preimage_bi `{Proset X, Proset Y} : Bimonotone (preimage (X:=X) (Y:=Y)).
+Proof. move=> [F ?] [G ?] /= D ? ? -> //. Qed.
+Instance Map_fmp `{Proset X, Proset Y} (F : Map X Y)
+  : FrameMorphPacked (preimage F) := proj2_sig _.
+Definition in_Map {X Y} `{FrameMorph Y X F} : Map X Y := F ↾ FMP.
+Arguments in_Map {_ _ _ _ _ _} F {_ _ _ _} /.
+Instance: Params (@in_Map) 6 := {}.
+Lemma preimage_in_Map `{FrameMorph Y X F}
+  : (in_Map F)⁻¹ = F.
+Proof. done. Qed.
+(* WARNING: This is brittle. It won't work in cases where the implicit arguments are filled
+            differently from how Coq has inferred them here. *)
+Lemma in_Map_preimage `{Proset X, Proset Y} {F : Map X Y} : in_Map F⁻¹ = F.
+Proof. case: F => F [*] //=. Qed.
+Lemma Map_core `{Proset X, Proset Y} {F G : Map X Y} : (forall A, F⁻¹ A ⟛ G⁻¹ A) <-> F ⟛ G.
+Proof. compute; firstorder. Qed.
+Definition Map_id `{Proset X} : Map X X := in_Map id.
+Definition Map_compose `{Proset X, Proset Y, Proset Z'}
+           (F : Map Y Z') (G : Map X Y) : Map X Z' := in_Map (G⁻¹ ∘ F⁻¹).
+Infix "⊚" := Map_compose (at level 40) : proset_scope.
+Notation "( f ⊚.)" := (Map_compose f) (only parsing) : proset_scope.
+Notation "(.⊚ f )" := (flip Map_compose f) (only parsing) : proset_scope.
+Instance: Params (@Map_id) 3 := {}.
+Instance: Params (@Map_compose) 9 := {}.
+Instance Map_compose_bi `{Proset X, Proset Y, Proset Z'}
+  : Bimonotone (Map_compose (X:=X) (Y:=Y) (Z':=Z')).
+Proof. move=> f g D f' g' D' x /=; rewrite D D' //. Qed.
+Lemma Map_id_lident `{Proset X, Proset Y} {F : Map X Y}
+  : Map_id ⊚ F ⟛ F.
+Proof. compute; by fold (pro_le (X:=X)). Qed.
+Lemma Map_id_rident `{Proset X, Proset Y} {F : Map X Y}
+  : F ⊚ Map_id ⟛ F.
+Proof. compute; by fold (pro_le (X:=X)). Qed.
+Lemma Map_compose_assoc `{Proset X, Proset Y, Proset Z', Proset W}
+      {F : Map Z' W} {G : Map Y Z'} {H' : Map X Y}
+  : F ⊚ (G ⊚ H') ⟛ (F ⊚ G) ⊚ H'.
+Proof. compute; by fold (pro_le (X:=X)). Qed.
+Definition preimage_of `{Proset X, Proset Y} (y : Y) : Map X Y -> X := fun F => F⁻¹ y.
+Arguments preimage_of {_ _ _ _ _ _} y _ /.
+Instance: Params (@preimage_of) 6 := {}.
+Instance preimage_of_mono `{Proset X, Proset Y}
+  : Monotone (preimage_of (X:=X) (Y:=Y)).
+Proof. solve_proper. Qed.
+Instance preimage_of_bi `{Proset X, Proset Y}
+  : Bimonotone (preimage_of (X:=X) (Y:=Y)).
+Proof. solve_proper. Qed.
+Instance preimage_of_cocontinuous `{Proset X, Proset Y, !SupLattice X}
+  : Cocontinuous (preimage_of (X:=X) (Y:=Y)).
+Proof.
+  move=> R J.
+  apply/preserves_sup_alt => ?; apply/sup_unique/pw_core' => f /=.
+  rewrite distrib_sup //.
+Qed.
+Instance preimage_of_lex `{Proset X, Proset Y, !MeetSemilattice X}
+  : Lex (preimage_of (X:=X) (Y:=Y)).
+Proof.
+  move=> R ? ? J.
+  apply/preserves_inf_alt => ?; apply/inf_unique/pw_core' => f /=.
+  rewrite distrib_inf //.
+Qed.
+
+
+(* The point as a locale. *)
+Definition point : Type := Prop.
+
+Instance embed_prop_lex `{Frame X} : Lex (embed_prop (X:=X)).
+Proof.
+  apply: lex_alt => J; apply: distrib_inf_sufficient.
+  - apply: embed_prop_right => -[].
+  - apply: prop_loop => [| ?] ; first apply: (inf_lb true).
+    apply: prop_loop => [| ?] ; first apply: (inf_lb false).
+    apply: embed_prop_right => -[] //.
+Qed.
+Definition to_point `{Frame X} : Map X point := in_Map embed_prop.
+Instance: Params (@to_point) 7 := {}.
+Lemma point_terminal `{Frame X} (F : Map X point) : F ⟛ to_point.
+Proof.
+  apply/Map_core => p.
+  rewrite {1}(mono_core F⁻¹ (_ : p ⟛ (Sup H : p, ⊤))).
+  - rewrite distrib_sup.
+    apply: (mono_core esup); apply/pw_core' => ?; apply: distrib_top.
+  - split; last by firstorder.
+    move=> H_p; exists H_p => -[].
+Qed.
+
+(* TODO Put this in the right place. *)
+Program Instance Hom_exponents `{Proset X, Proset Y, !InfLattice Y, !Exponents Y}
+  : Exponents (Hom X Y)
+  := {| exponential F G A := Inf B : {B0 | A ⊢ B0}, F (` B) ⟿ G (` B) |}.
+Next Obligation.
+  move=> * A B D.
+  apply: inf_right => -[B' D'] /=.
+  apply: (inf_left (_ ↾ _)); by etransitivity.
+Qed.
+Next Obligation.
+  move=> X ? ? Y ? ? ? ? F G H; split.
+  - move=> Uncurried A /=; apply: inf_right => -[B /= ->].
+    rewrite -meet_exponential -(distrib_meet (F:=Hom_eval_at B)); apply/Uncurried.
+  - move=> /= Curried A; specialize (Curried A); simpl in Curried.
+    setoid_rewrite (inf_lb (A ↾ reflexivity _)) in Curried; simpl in Curried.
+    etransitivity; first by apply: (F_meet (F:=Hom_eval_at A)).
+    rewrite meet_exponential //.
+Qed.
+
+Definition sier : Type := Hom bool Prop.
+Identity Coercion sier_to_Hom : sier >-> Hom.
+Definition characteristic_f `{Frame X} (U : X) (S : sier) : X
+  := (embed_prop (S true) ⩕ U) ⩖ embed_prop (S false).
+Arguments characteristic_f {_ _ _ _ _ _ _} U S /.
+Instance: Params (@characteristic_f) 7 := {}.
+Lemma characteristic_f_uni `{Frame X} (U : X) (S : sier) (V : X)
+  : characteristic_f U S ⊢ V <-> (S true -> U ⊢ V) /\ (S false -> ⊤ ⊢ V).
+Proof.
+  split.
+  - move=> /= <-; split=> H_S.
+    + apply: join_right1; apply: meet_right; [by apply: embed_prop_right | done].
+    + apply: join_right2; by apply: embed_prop_right.
+  - move=> [D1 D2]; apply: join_left.
+    + apply: (prop_loop meet_proj1) => /D1 ->; apply: meet_proj2.
+    + by apply: embed_prop_left.
+Qed.
+(*
+Lemma characteristic_f_cases `{Frame X} (U : X) (S : sier)
+  : characteristic_f U S ⊢ ⌜ (S false /\ ⊤ ⟛ characteristic_f U S) \/
+                             (S true /\ U ⊢ characteristic_f U S) ⌝.
+Proof.
+  apply: join_left.
+  - apply: sup_left => ?; apply: embed_prop_right.
+    right; split; first by done.
+    apply: join_right1; by apply: sup_ub.
+  - apply: mono => ?.
+    left; split; first by done.
+    split; [apply: join_right2; by apply: embed_prop_right | apply: top_right].
+Qed.
+*)
+Instance characteristic_f_bi `{Frame X} : Bimonotone (characteristic_f (X:=X)).
+Proof. solve_proper. Qed.
+Instance characteristic_f_cocontinuous `{Frame X} {U : X}
+  : Cocontinuous (characteristic_f U).
+Proof.
+  move=> R J; apply: distrib_sup_sufficient.
+  apply/characteristic_f_uni; split=> -[r /= ?]; apply: (sup_right r).
+  + apply: join_right1; apply: meet_right; [by apply: embed_prop_right | done].
+  + apply: join_right2; by apply: embed_prop_right.
+Qed.
+Instance characteristic_f_lex `{Frame X} {U : X}
+  : Lex (characteristic_f U).
+Proof.
+  apply: lex_alt => J; apply: distrib_inf_sufficient.
+  - apply: join_right2; apply: embed_prop_right => -[].
+  - rewrite [L in L ⊢ _](meet_right (reflexivity _) (reflexivity _))
+            {1}(inf_lb false) (inf_lb true) meet_exponential.
+    apply/characteristic_f_uni; split => H_J1.
+    all: rewrite -meet_exponential l_meet_exponential.
+    all: apply/characteristic_f_uni; split => H_J2; rewrite -l_meet_exponential.
+    + apply: join_right1; apply: meet_right.
+      * apply: embed_prop_right; by case.
+      * apply: meet_proj1.
+    + apply: join_right1; apply: meet_right.
+      * apply: embed_prop_right; case=> //=; by apply: (Hom_mono (J true)) H_J2.
+      * apply: meet_proj1.
+    + apply: join_right1; apply: meet_right.
+      * apply: embed_prop_right; case=> //=; by apply: (Hom_mono (J false)) H_J1.
+      * apply: meet_proj2.
+    + apply: join_right2; apply: embed_prop_right; by case.
+Qed.
+
+(*
+    apply: (prop_loop (R:=J true true)) => [| H_J1]. {
+      apply: (inf_left true).
+      apply: join_left; apply: sup_left => H_J; apply: embed_prop_right; first by done.
+      move: H_J; by apply: (Hom_mono (J true)).
+    }
+    apply: (prop_loop (R:=J false true)) => [| H_J2]. {
+      apply: (inf_left false).
+      apply: join_left; apply: sup_left => H_J; apply: embed_prop_right; first by done.
+      move: H_J; by apply: (Hom_mono (J false)).
+    }
+    apply: join_right1.  simpl. unfold flip. ; apply: embed_prop_right => -[] //=.
+Qed.
+*)
+Definition characteristic `{Frame X} (U : X) : Map X sier
+  := in_Map (characteristic_f U).
+Arguments characteristic {_ _ _ _ _ _ _} U.
+Instance: Params (@characteristic) 7 := {}.
+Instance characteristic_mono `{Frame X} : Monotone (characteristic (X:=X)).
+Proof. move=> U V D /= S; rewrite D //. Qed.
+Definition universal_open : sier := in_Hom is_top.
+Theorem sier_classifies_opens `{Frame X} (U : X) (F : Map X sier)
+  : F ⟛ characteristic U <-> F⁻¹ universal_open ⟛ U.
+Proof.
+  split.
+  - move=> -> /=; split; first apply: join_left.
+    + apply: meet_proj2.
+    + apply: embed_prop_left => ? //.
+    + apply: join_right1; apply: meet_right => //; by apply: embed_prop_right.
+  - move=> <- /=; apply/Map_core => S /=.
+    rewrite (mono_core (F⁻¹) (_ : S ⟛ (characteristic universal_open)⁻¹ S)).
+    + rewrite distrib_join distrib_meet distrib_embed_prop.
+      apply: mono_core; apply: distrib_embed_prop.
+    + apply/Hom_core => b.
+      rewrite -[R in _ ⟛ R]/(Hom_eval_at b _)
+        distrib_join distrib_meet [_ _ universal_open]/= /is_top.
+      split.
+      * case: b.
+        -- apply join_right1, meet_right => // H_S; exists H_S => -[].
+        -- apply join_right2 => H_S; exists H_S => -[].
+      * apply join_left => [P | [H_S _]].
+        -- move: (P true) (P false) => [? ?] <- //.
+        -- case: b => //; by apply: (Hom_mono S) H_S.
+Qed.
+
+Definition point_of (X : Type) `{Proset X} : Type := Map point X.
+Definition point_set (X : Type) `{Proset X} : Type := point_of X -> Prop.
+Definition points_in `{Proset X} : X -> point_set X
+  := preimage_of.
+Arguments points_in {_ _ _} U !_ /.
+Instance: Params (@points_in) 3 := {}.
+Definition frame_interior `{Proset X, !SupLattice X} : point_set X -> X
+  := universal_right_adjoint points_in.
+Arguments frame_interior {_ _ _ _} U /.
+Instance: Params (@frame_interior) 4 := {}.
+Instance frame_interior_mono `{Proset X, !SupLattice X}
+  : Monotone (frame_interior (X:=X)).
+Proof. move=> U V D; rewrite /frame_interior D //. Qed.
+Instance points_in_frame_interior_adj `{Proset X, !SupLattice X}
+  : points_in (X:=X) ⊣ frame_interior
+  := universal_adjunction2.
+Definition interior `{Proset X, !SupLattice X} : point_set X -> point_set X
+  := points_in ∘ frame_interior.
+Arguments interior {_ _ _ _} U /.
+Instance: Params (@interior) 4 := {}.
+
+Definition open `{Proset X} (U : point_set X) : Prop
+  := exists V, U ⟛ points_in V.
+Lemma open_alt `{Frame X} (U : point_set X)
+  : open U <-> forall p, U p -> exists V, points_in V p /\ points_in V ⊢ U.
+Proof.
+  split; first by firstorder.
+  move=> Cov; exists (frame_interior U); split; last by apply: (adj_counit' _ _).
+  move=> p /=; rewrite -[R in _ ⊢ R]F_sup => U_p /=.
+  move: (U_p) => /Cov [V D] /=.
+  unshelve eexists (V ↾ _) => /=; firstorder.
+Qed.
+
+(* TODO Move this
+Definition choose `{Proset X, !SupLattice X} (P : X -> Prop) : X := Sup A : sig P, `A.
+Lemma choose_spec `{Proset X, !SupLattice X} (P : X -> Prop) `{!Monotone P}
+  : (exists A, P A) -> P (choose P).
+Proof. move=> [A PA]; rewrite /choose -(sup_ub (A ↾ PA)) //=. Qed.
+Theorem choice `{Proset X, !SupLattice X} {R} (P : R -> X -> Prop)
+        `{!Proper ((=) ==> (⊢) ==> impl) P}
+  : (forall r, exists A, P r A) -> exists f, forall r, P r (f r).
+Proof. move=> AllEx; exists (fun r => choose (P r)) => r; by apply: choose_spec. Qed.
+*)
+
+Lemma open_union `{Frame X} {R} (J : R -> point_set X)
+  : (forall r, open (J r)) -> open (sup J).
+Proof.
+  move=> AllOpen.
+  apply/open_alt => p [r /= In].
+  case: (AllOpen r) => U E; exists U; firstorder.
+Qed.
+Lemma open_intersection `{Frame X, Finite R} (J : R -> point_set X)
+  : (forall r, open (J r)) -> open (inf J).
+Proof.
+  move=> /finite_choice [Neighs E_Neighs].
+  apply/open_alt => p /= InAll.
+  exists (inf Neighs); split; rewrite distrib_inf; firstorder.
+Qed.
+
+Definition soberification (X : Type) `{Proset X} : Type
+  := @sig (point_set X) open.
+Definition as_open `{Proset X, !SupLattice X} : soberification X -> X
+  := frame_interior ∘ sval.
+Arguments as_open {_ _ _ _} U /.
+Instance: Params (@as_open) 4 := {}.
+Instance as_open_mono `{Frame X} : Monotone (as_open (X:=X)).
+Proof. unfold as_open; typeclasses eauto. Qed.
+(*
+Instance as_open_reflecting `{Frame X} : Reflecting (as_open (X:=X)).
+*)
+
+Program Instance soberification_suplattice `{Frame X} : SupLattice (soberification X)
+  := fun R J => {| sup := sup (sval ∘ J) ↾ _ |}.
+Next Obligation. move=> *; apply: open_union => r /=; apply: proj2_sig. Qed.
+Next Obligation. move=> *; apply/(reflecting_reflects_sup (F:=sval))/is_sup. Qed.
+Program Instance soberification_meet_semilattice `{Frame X}
+  : MeetSemilattice (soberification X)
+  := fun R _ _ J => {| inf := inf (sval ∘ J) ↾ _ |}.
+Next Obligation. move=> *; apply: open_intersection => r /=; apply: proj2_sig. Qed.
+Next Obligation. move=> *; apply/(reflecting_reflects_inf (F:=sval))/is_inf. Qed.
+(*
+Program Instance soberification_exponents `{Frame X} : Exponents (soberification X)
+  := {| exponential U V := points_in (frame_interior U ⟿ frame_interior V) |}.
+Next Obligation. firstorder. Qed.
+*)
